value_is_nf

plf/Types.v
@@ -4,3 +4,117 @@ From PLF Require Import Maps.
 From PLF Require Import Smallstep.
 Set Default Goal Selector "!".
 Hint Constructors multi : core.
+
+Module TM.
+Inductive tm : Type :=
+  | tru : tm
+  | fls : tm
+  | ite : tm -> tm -> tm -> tm
+  | zro : tm
+  | scc : tm -> tm
+  | prd : tm -> tm
+  | iszro : tm -> tm.
+
+Declare Custom Entry tm.
+Declare Scope tm_scope.
+Notation "'true'" := true (at level 1): tm_scope.
+Notation "'true'" := (tru) (in custom tm at level 0): tm_scope.
+Notation "'false'" := false (at level 1): tm_scope.
+Notation "'false'" := (fls) (in custom tm at level 0): tm_scope.
+Notation "<{ e }>" := e (e custom tm at level 99): tm_scope.
+Notation "( x )" := x (in custom tm, x at level 99): tm_scope.
+Notation "x" := x (in custom tm at level 0, x constr at level 0): tm_scope.
+Notation "'0'" := (zro) (in custom tm at level 0): tm_scope.
+Notation "'0'" := 0 (at level 1): tm_scope.
+Notation "'succ' x" := (scc x) (in custom tm at level 90, x custom tm at level 80): tm_scope.
+Notation "'pred' x" := (prd x) (in custom tm at level 90, x custom tm at level 80): tm_scope.
+Notation "'iszero' x" := (iszro x) (in custom tm at level 80, x custom tm at level 70): tm_scope.
+Notation "'if' c 'then' t 'else' e" := (ite c t e)
+                 (in custom tm at level 90, c custom tm at level 80,
+                  t custom tm at level 80, e custom tm at level 80): tm_scope.
+Local Open Scope tm_scope.
+
+Inductive bvalue : tm -> Prop :=
+  | bv_True : bvalue <{ true }>
+  | bv_false : bvalue <{ false }>.
+Inductive nvalue : tm -> Prop :=
+  | nv_0 : nvalue <{ 0 }>
+  | nv_succ : forall t, nvalue t -> nvalue <{ succ t }>.
+Definition value (t : tm) := bvalue t \/ nvalue t.
+Hint Constructors bvalue nvalue : core.
+Hint Unfold value : core.
+
+Reserved Notation "t '-->' t'" (at level 40).
+Inductive step : tm -> tm -> Prop :=
+  | ST_IfTrue : forall t1 t2,
+      <{ if true then t1 else t2 }> --> t1
+  | ST_IfFalse : forall t1 t2,
+      <{ if false then t1 else t2 }> --> t2
+  | ST_If : forall c c' t2 t3,
+      c --> c' ->
+      <{ if c then t2 else t3 }> --> <{ if c' then t2 else t3 }>
+  | ST_Succ : forall t1 t1',
+      t1 --> t1' ->
+      <{ succ t1 }> --> <{ succ t1' }>
+  | ST_Pred0 :
+      <{ pred 0 }> --> <{ 0 }>
+  | ST_PredSucc : forall v,
+      nvalue v ->
+      <{ pred (succ v) }> --> v
+  | ST_Pred : forall t1 t1',
+      t1 --> t1' ->
+      <{ pred t1 }> --> <{ pred t1' }>
+  | ST_Iszero0 :
+      <{ iszero 0 }> --> <{ true }>
+  | ST_IszeroSucc : forall v,
+       nvalue v ->
+      <{ iszero (succ v) }> --> <{ false }>
+  | ST_Iszero : forall t1 t1',
+      t1 --> t1' ->
+      <{ iszero t1 }> --> <{ iszero t1' }>
+
+where "t '-->' t'" := (step t t').
+Hint Constructors step : core.
+
+Notation step_normal_form := (normal_form step).
+Definition stuck (t : tm) : Prop :=
+  step_normal_form t /\ ~ value t.
+Hint Unfold stuck : core.
+
+Example some_term_is_stuck :
+  exists t, stuck t.
+Proof.
+  exists <{ iszero false }>.
+  unfold stuck. split.
+  - unfold step_normal_form. unfold not.
+    intros. destruct H as [t1 H]. inversion H. inversion H1.
+  - unfold not. intros. inversion H.
+    * inversion H0.
+    * inversion H0.
+Qed.
+
+Lemma value_is_nf : forall t,
+  value t -> step_normal_form t.
+Proof.
+  intros t H. inversion H.
+  - destruct H0.
+    + unfold step_normal_form.
+      unfold not. intros. destruct H0 as [t1 H0].
+      inversion H0.
+      + unfold step_normal_form.
+      unfold not. intros. destruct H0 as [t1 H0].
+      inversion H0.
+      - induction H0.
+      + unfold step_normal_form.
+        unfold not. intros. destruct H0 as [t1 H0].
+        inversion H0.
+      + unfold step_normal_form.
+        unfold not. intros.
+        inversion H0. 
+        * destruct H1 as [t' H1].
+          rewrite <- H2 in H1. inversion H1. inversion H4.
+        * destruct H1 as [t' H1]. clear H1.
+          inversion H2; clear H2.
+          ** rewrite <- H1 in H3.
+          rewrite <- H3 in IHnvalue.
+Admitted.
